\documentclass{beamer}

\usepackage{amssymb}
\usepackage{amsfonts}
\usepackage{amsmath}
\usepackage{amsthm}
\usepackage{setspace}
\usepackage{longtable}
\usepackage{graphicx}
\usepackage{mathtools}
\usepackage{color}
\usepackage{array}
\usepackage{calc} 
\usepackage{bm}
\usepackage{caption}
\usepackage{float}

\usetheme{CambridgeUS}
\useoutertheme{infolines}
%numbering
\setbeamercolor{background canvas}{bg=white}
\setbeamersize{text margin left=1cm,text margin right=1cm}

\title[AI1110  Assignment-9]{ASSIGNMENT-9}
\subtitle{AI1110}
\author[]{MUKUNDA REDDY \\ AI21BTECH11021}
\date

\begin{document}
  \begin{frame}
      \titlepage
  \end{frame}
  
  \begin{frame}{Outline}
      \tableofcontents
  \end{frame}
  
  \section{Question}
  \begin{frame}{Exercise 9-39}
  Find autocorrelation $R(\tau)$ ? if \\
  \begin{center}
  \begin{enumerate}[a]
      \item $S(w) = \frac{1}{(1+w^{4})}$
      \item $S(w) = \frac{1}{(4+w^{2})^{2}}$
  \end{enumerate}
  \end{center}
  \end{frame}
  
  \section{Solution}
  \subsection{Solution (a)}
  \begin{frame}{Solution (a)}
  \begin{align*}
      S(s)  &= \frac{1}{1+s^{4}}  \\
         &=  \frac{1}{(s^{2}+\sqrt{2}s+1)(s^{2}-\sqrt{2}s+1)}  \\
  \end{align*}
     Now we know that for the equation of kind
     $y\prime\prime(t) +b y\prime(t) +cy(t) = x(t),
     S_{xx} (w) = q$ Then
     $$ S_{yy} (w) = \frac{q}{(c-w^{2})^{2}+b^{2}w^{2}} $$
  \end{frame}

   \begin{frame}{Solution (a)}
       This is a special case with $b = \sqrt{2},c = 1$
       i.e. $b^{2} < 4c$ so we have autocorrelation as
       $$ R_{yy} ( \tau) = \frac{q}{2bc}e^{-\alpha |\tau|} \left( cos(\beta \tau) + \frac{\alpha}{\beta}sin(\beta |\tau|) \right),\alpha = \frac{b}{2} , {\alpha}^{2} + {\beta}^{2} = c $$
       Subtituting we get 
       $$R(\tau) = \frac{1}{2\sqrt{2}}e^{\frac{-|\tau|}{\sqrt{2}}}\left( cos(\frac{\tau}{\sqrt{2}}) + sin(\frac{|\tau|}{\sqrt{2}} ) \right)$$
   \end{frame}
   
  \subsection{Solution (b)}
  \begin{frame}{Solution (b)}
      From the pair $e^{-2|\tau|} \xleftrightarrow \ \frac{4}{4+w^{2}}$ and it follows that
      $e^{-2|\tau|}*e^{-2|\tau|} \xleftrightarrow \ \frac{16}{(4+w^{2})^{2}}$ hence for $\tau>0$
      \begin{align*}
          16 R(\tau) &= \int_{-\infty}^{\infty} e^{-2|x|}e^{-2|\tau-x|} dx  \\
          &= \int_{-\infty}^{0} e^{-2x}e^{-2(\tau-x)} dx +\int_{0}^{\tau} e^{-2x}e^{-2(\tau-x)} dx  \\
          &+ \int_{\tau}^{\infty} e^{-2x}e^{2(\tau-x)} dx \\
          &=  \frac{1}{2}e^{-2\tau}(1+2\tau)
      \end{align*}
  \end{frame}
  
  \begin{frame}{Solution (b)}
      after simplification we are left with the autocorrelation ,
      $$R (\tau) = \frac{1}{32}e^{-2\tau}(1+2\tau) $$
  \end{frame}
  
\end{document}
